cbor_det_serialize_string (necessary for CDDL .cbordet)

src/cbor/pulse/CBOR.Pulse.API.Base.fst
@@ -1553,6 +1553,44 @@ let cbor_det_serialize_array_t =
     pure (cbor_det_serialize_array_postcond l res v)
   )
 
+let cbor_det_serialize_string_precond
+  (ty: major_type_byte_string_or_text_string)
+  (off: U64.t)
+  (v: Seq.seq U8.t)
+: Tot prop
+= U64.v off <= Seq.length v /\
+  (ty == cbor_major_type_text_string ==> CBOR.Spec.API.UTF8.correct (Seq.slice v 0 (U64.v off)))
+
+let cbor_det_serialize_string_postcond
+  (ty: major_type_byte_string_or_text_string)
+  (off: U64.t)
+  (v: Seq.seq U8.t)
+  (res: SZ.t)
+  (v': Seq.seq U8.t)
+: Tot prop
+= cbor_det_serialize_string_precond ty off v /\
+  begin let l = Seq.slice v 0 (U64.v off) in
+  Seq.length v' == Seq.length v /\
+  SZ.v res <= Seq.length v' /\
+  (res == 0sz <==> Seq.length (Spec.cbor_det_serialize (pack (CString ty l))) > Seq.length v') /\
+  (SZ.v res > 0 ==> Seq.slice v' 0 (SZ.v res) `Seq.equal` Spec.cbor_det_serialize (pack (CString ty l)))
+  end
+
+inline_for_extraction
+let cbor_det_serialize_string_t =
+  (ty: major_type_byte_string_or_text_string) ->
+  (off: U64.t) ->
+  (out: S.slice U8.t) ->
+  (#v: Ghost.erased (Seq.seq U8.t)) ->
+  stt SZ.t
+  (pts_to out v **
+    pure (cbor_det_serialize_string_precond ty off v)
+  )
+  (fun res -> exists* v' .
+    pts_to out v' **
+    pure (cbor_det_serialize_string_postcond ty off v res v')
+  )
+
 let cbor_det_serialize_map_insert_pre
   (m: cbor_map)
   (off2: SZ.t)
